code/ecdsap256/Hacl.Impl.P256.ECDSA.Defensive.fst
@@ -38,6 +38,92 @@ open Spec.Hash.Definitions
 
 open Hacl.Impl.ECDSA.P256.Signature.Agile
 
+open Lib.IntTypes.Intrinsics
+
+
+open Lib.Memzero
+
+#set-options "--fuel 0 --ifuel 0 --z3rlimit 200"
+
+val cleanUpCritical: critical : lbuffer uint64 (size 4) -> Stack unit
+  (requires fun h -> live h critical)
+  (ensures fun h0 _ h1 -> modifies (loc critical) h0 h1 /\ as_seq h1 critical == Seq.create 4 (u64 0))
+
+let cleanUpCritical critical =
+  clear_words_u64 4ul critical
+
+
+val sub4: x: felem ->  result: felem -> 
+  Stack uint64
+    (requires fun h -> live h x /\ live h result /\ disjoint x result)
+    (ensures fun h0 c h1 -> modifies (loc result) h0 h1 /\ 
+      (if (nat_from_intseq_be (as_seq h0 x) >= prime_p256_order) 
+	then uint_v c = 0 
+	else uint_v c = 1))
+
+let sub4 x result = 
+  let h0 = ST.get() in 
+    let r0 = sub result (size 0) (size 1) in 
+    let r1 = sub result (size 1) (size 1) in 
+    let r2 = sub result (size 2) (size 1) in 
+    let r3 = sub result (size 3) (size 1) in 
+
+    recall_contents prime256order_buffer (Lib.Sequence.of_list p256_order_prime_list);
+
+    let cc0 = sub_borrow_u64 (u64 0) x.(size 3) prime256order_buffer.(size 0) r0 in 
+      let h1 = ST.get() in 
+    let cc1 = sub_borrow_u64 cc0 x.(size 2) prime256order_buffer.(size 1) r1 in 
+      let h2 = ST.get() in 
+    let cc2 = sub_borrow_u64 cc1 x.(size 1) prime256order_buffer.(size 2) r2 in 
+      let h3 = ST.get() in 
+    let cc3 = sub_borrow_u64 cc2 x.(size 0) prime256order_buffer.(size 3) r3 in 
+      let h4 = ST.get() in 
+
+    
+    let open Lib.Sequence in 
+
+    nat_from_intseq_be_slice_lemma (as_seq h0 x) 3; 
+    nat_from_intseq_be_slice_lemma (slice (as_seq h0 x) 0 3) 2;
+    nat_from_intseq_be_slice_lemma (slice (as_seq h0 x) 0 2) 1; 
+    
+    nat_from_intseq_be_lemma0 (slice (as_seq h0 x) 3 4);
+    nat_from_intseq_be_lemma0 (slice (as_seq h0 x) 2 3);
+    nat_from_intseq_be_lemma0 (slice (as_seq h0 x) 1 2);
+    nat_from_intseq_be_lemma0 (slice (as_seq h0 x) 0 1);
+
+    assert(disjoint prime256order_buffer result);
+
+    cc3
+    
+
+inline_for_extraction noextract
+val lessThanOrderU8: i: lbuffer uint8 (size 32) -> critical: lbuffer uint64 (size 4) -> critical1: lbuffer uint64 (size 4) -> Stack uint64 
+  (requires fun h -> live h i /\ live h critical /\ live h critical1 /\ disjoint i critical /\ disjoint critical critical1)
+  (ensures fun h0 r h1 -> modifies (loc critical |+| loc critical1) h0 h1 /\ (uint_v r == 0 <==> nat_from_bytes_be (as_seq h0 i) < prime_p256_order))
+
+let lessThanOrderU8 i critical critical1 = 
+    let h0 = ST.get() in 
+  toUint64 i critical;
+    let h1 = ST.get() in 
+    Lib.ByteSequence.uints_from_bytes_be_nat_lemma #U64 #_ #4 (as_seq h0 i);
+    
+  let carry = sub4 critical  critical1 in 
+  let less = eq_mask carry (u64 0) in 
+  eq_mask_lemma carry (u64 0);
+  less
+
+
+(* This function is not SC resistant *)
+val compareTo0TwoVariablesNotSC: a: uint64 -> b: uint64 ->
+  Tot (r : bool {r = (uint_v a = 0 && uint_v b = 0)})
+
+let compareTo0TwoVariablesNotSC a b = 
+  let open Hacl.Impl.P256.LowLevel.RawCmp in 
+  let firstZero = eq_0_u64 a in 
+  let secondZero = eq_0_u64 b in 
+  firstZero && secondZero
+
+
 
 
 inline_for_extraction noextract
@@ -47,17 +133,16 @@ val ecdsa_sign_p256_sha2_def: alg: hash_alg_ecdsa
   -> m: lbuffer uint8 mLen 
   -> privKey: lbuffer uint8 (size 32) 
   -> k: lbuffer uint8 (size 32) -> 
-  Stack uint64
+  Stack bool
   (requires fun h -> 
     live h result /\ live h m /\ live h privKey /\ live h k /\
     disjoint result m /\
     disjoint result privKey /\
-    disjoint result k /\
-    nat_from_bytes_be (as_seq h privKey) < prime_p256_order /\
-    nat_from_bytes_be (as_seq h k) < prime_p256_order
+    disjoint result k 
   )
   (ensures fun h0 flag h1 -> 
     modifies (loc result) h0 h1 /\
+      if 
      (assert_norm (pow2 32 < pow2 61);
       let resultR = gsub result (size 0) (size 32) in 
       let resultS = gsub result (size 32) (size 32) in 
@@ -69,4 +154,26 @@ val ecdsa_sign_p256_sha2_def: alg: hash_alg_ecdsa
   )
 
 
-let ecdsa_sign_p256_sha2_def alg result mLen m privKey k = ecdsa_signature alg result mLen m privKey k
+let ecdsa_sign_p256_sha2_def alg result mLen m privKey k = 
+  push_frame();
+  let crTemp = create (size 8) (u64 0) in 
+  let cr0 = sub crTemp (size 0) (size 4) in 
+  let cr1 = sub crTemp (size 4) (size 4) in  
+    
+  let less0 = lessThanOrderU8 privKey cr0 cr1 in 
+  let less1 = lessThanOrderU8 k cr0 cr1 in 
+  let flagLessOrder = compareTo0TwoVariablesNotSC less0 less1 in 
+
+  if not flagLessOrder then 
+    begin 
+      admit();
+      pop_frame();
+      false
+    end
+  else
+    begin
+    let r = ecdsa_signature alg result mLen m privKey k in 
+    admit();
+    pop_frame();
+    r
+    end
