code/ecdsap256/Hacl.P256.fsti
@@ -403,30 +403,15 @@ val isMoreThanZeroLessThanOrder: x: lbuffer uint8 (size 32) -> Stack uint64
 
 
 
-
-
-
-
-
-
-
-
-
-
-
-
-
-
 [@ (Comment " Input: result buffer: uint8[64], \n m buffer: uint8 [mLen], \n priv(ate)Key: uint8[32], \n k (nonce): uint32[32]. 
   \n Output: uint64, where 0 stands for the correct signature generation. All the other values mean that an error has occurred. 
   \n The private key and the nonce are expected to be less than the curve order.")]
-
 val ecdsa_sign_p256_sha2_def: result: lbuffer uint8 (size 64) 
   -> mLen: size_t 
   -> m: lbuffer uint8 mLen 
   -> privKey: lbuffer uint8 (size 32) 
   -> k: lbuffer uint8 (size 32) -> 
-  Stack uint64
+  Stack bool
   (requires fun h -> 
     live h result /\ live h m /\ live h privKey /\ live h k /\
     disjoint result m /\
@@ -437,12 +422,13 @@ val ecdsa_sign_p256_sha2_def: result: lbuffer uint8 (size 64)
   )
   (ensures fun h0 flag h1 -> 
     modifies (loc result) h0 h1 /\
-     (assert_norm (pow2 32 < pow2 61);
-      let resultR = gsub result (size 0) (size 32) in 
-      let resultS = gsub result (size 32) (size 32) in 
-      let r, s, flagSpec = Spec.ECDSA.ecdsa_signature_agile (Spec.ECDSA.Hash SHA2_256) (uint_v mLen) (as_seq h0 m) (as_seq h0 privKey) (as_seq h0 k) in 
-      as_seq h1 resultR == nat_to_bytes_be 32 r /\
-      as_seq h1 resultS == nat_to_bytes_be 32 s /\
-      flag == flagSpec 
-    )    
-
+     (
+       assert_norm (pow2 32 < pow2 61);
+       let resultR = gsub result (size 0) (size 32) in 
+       let resultS = gsub result (size 32) (size 32) in 
+       let r, s, flagSpec = Spec.ECDSA.ecdsa_signature_agile (Spec.ECDSA.Hash SHA2_256) (uint_v mLen) (as_seq h0 m) (as_seq h0 privKey) (as_seq h0 k) in 
+       as_seq h1 resultR == nat_to_bytes_be 32 r /\
+       as_seq h1 resultS == nat_to_bytes_be 32 s /\
+       flag == flagSpec 
+    )   
+)
